src/specs/seq.fst
@@ -13,87 +13,82 @@
 // 
 // ,$
 
-module Tesseract.Specs.Seq
+//@requires "fstar:ext.fst"
 
-   type _spec_g (item_t: Type) =
-      nat -> Tot (option item_t)
+module Tesseract.Specs.Seq
 
    type _seq_g (item_t: Type) 
       = 
          { 
-            spec: _spec_g item_t;
+            maybe_nth: nat -> Tot (option item_t);
             length: nat
          }
 
-   type is_seq_safe: #item_t: Type -> spec: _spec_g item_t -> length: nat -> Type 
-      =
-         fun (item_t: Type) (spec: _spec_g item_t) (length: nat) ->
-            forall (idx: nat).
-               ((idx < length) <==> (is_Some (spec idx)))
-               /\ ((idx >= length) <==> (None = (spec idx)))
+   type is_seq_safe: #item_t: Type -> seq: _seq_g item_t -> Type 
+      = fun (item_t: Type) (seq: _seq_g item_t) ->
+         forall (index: nat).
+            ((index < seq.length) <==> (is_Some (seq.maybe_nth index)))
+            /\ ((index >= seq.length) <==> (None = (seq.maybe_nth index)))
 
    type seq_g (item_t: Type) 
-      = seq: _seq_g item_t{is_seq_safe seq.spec seq.length}
+      = seq: _seq_g item_t{is_seq_safe seq}
 
-   val bless:
-      #item_t: Type ->
-      spec: _spec_g item_t -> length: nat{is_seq_safe spec length} -> Tot (seq_g item_t)
-   let bless spec length 
-      =
-         {
-            spec = spec;
-            length = length
-         }
+   type index_g (#item_t: Type) (seq: seq_g item_t) 
+      = index: nat{index < seq.length}
+
+   val length: 
+      #item_t: Type 
+      -> seq_g item_t 
+      -> Tot nat
+   let length (item_t: Type) (seq: seq_g item_t)
+      = seq.length
+
+   type are_equal 
+      (#item_t: Type) 
+      (lhs: seq_g item_t) 
+      (rhs: seq_g item_t)
+      = (FunctionalExtensionality.FEq lhs.maybe_nth rhs.maybe_nth) 
+         /\ (lhs.length = rhs.length)
 
    val empty: #item_t: Type -> Tot (seq_g item_t)
    let empty (item_t: Type) 
-      = bless (fun _ -> None) 0
+      = {
+         maybe_nth = (fun _ -> None);
+         length = 0
+      }
 
-   val single: 
-      #item_t: Type -> 
-      item_t -> Tot (seq_g item_t)
+   val single: #item_t: Type -> item_t -> Tot (seq_g item_t)
    let single item 
-      =
-         bless
-            (fun idx ->
-               if 0 = idx then
+      = {
+         maybe_nth = 
+            (fun index ->
+               if 0 = index then
                   Some item
                else
-                  None)
-            1
+                  None);
+         length = 1
+      }
 
-   val length: 
-      #item_t: Type -> 
-      seq_g item_t -> Tot nat
-   let length (item_t: Type) seq 
-      = seq.length
-
-   let to_map seq = seq.spec
-   let lookup seq = seq.spec
+   let to_map seq = seq.maybe_nth
+   let lookup seq = seq.maybe_nth
 
    val nth: 
-      #item_t: Type -> 
-      seq: seq_g item_t -> idx: nat{idx < length seq} 
-         -> Tot item_t
-   let nth (item_t: Type) seq idx
+      #item_t: Type 
+      -> seq: seq_g item_t 
+      -> index: index_g seq
+      -> Tot item_t
+   let nth (item_t: Type) seq index
       = 
-         match lookup seq idx with
+         match lookup seq index with
             | Some item ->
                item
 
-   val first: 
-      #item_t: Type -> 
-         seq: seq_g item_t{0 < length seq} 
-         -> Tot item_t
-   let first (item_t: Type) seq 
-      = nth seq 0
-
    val last: 
-      #item_t: Type -> 
-         seq: seq_g item_t{0 < length seq} 
-         -> Tot item_t
+      #item_t: Type 
+      -> seq: seq_g item_t{0 < length seq} 
+      -> Tot (index_g seq)
    let last (item_t: Type) seq 
-      = nth seq ((length seq) - 1)
+      = (length seq) - 1
 
    val append:
       #item_t: Type 
@@ -101,14 +96,15 @@ module Tesseract.Specs.Seq
       -> item_t
       -> Tot (seq_g item_t)
    let append (item_t: Type) seq item 
-      =
-         bless
-            (fun idx -> 
-               if idx = seq.length then 
+      = {
+         maybe_nth =
+            (fun index -> 
+               if index = seq.length then 
                   Some item 
                else 
-                  lookup seq idx)
-            (seq.length + 1)
+                  lookup seq index);
+         length = (seq.length + 1)
+      }
 
    val insert:
       #item_t: Type
@@ -117,85 +113,106 @@ module Tesseract.Specs.Seq
       -> item_t 
       -> Tot (seq_g item_t)
    let insert (item_t: Type) seq before item
-      = 
-         bless
+      = {
+         maybe_nth =
             (fun n ->
                if n = before then
                   Some item
                else if n < before then
                   lookup seq n
                else
-                  lookup seq (n - 1))
-            (seq.length + 1)
+                  lookup seq (n - 1));
+         length = (seq.length + 1)
+      }
 
    val remove:
       #item_t: Type
       -> seq: seq_g item_t{0 < length seq}
-      -> idx: nat{idx < length seq}
+      -> index: index_g seq
       -> Tot (seq_g item_t)
-   let remove (item_t: Type) seq idx 
-      = 
-         bless
+   let remove (item_t: Type) seq index 
+      = {
+         maybe_nth =
             (fun n ->
-               if n < idx then
+               if n < index then
                   lookup seq n
                else
-                  lookup seq (n + 1))
-            (seq.length - 1)
+                  lookup seq (n + 1));
+         length = (seq.length - 1)
+      }
 
    val concat: 
       #item_t: Type
-      -> seq_g item_t -> seq_g item_t
+      -> seq_g item_t 
+      -> seq_g item_t
       -> Tot (seq_g item_t)
    let concat lhs rhs 
-      =
-         bless
-            (fun idx ->
-               if idx < lhs.length then
-                  lhs.spec idx
+      = {
+         maybe_nth =
+            (fun index ->
+               if index < lhs.length then
+                  lhs.maybe_nth index
                else
-                  rhs.spec (idx - lhs.length))
+                  rhs.maybe_nth (index - lhs.length));
+         length =
             (lhs.length + rhs.length)
+      }
 
    val _foldl__loop: 
-      #item_t: Type -> #accum_t: Type -> 
-      seq: seq_g item_t -> (accum_t -> item_t -> Tot accum_t) 
-         -> accum_t -> idx: nat{idx < length seq}
-         -> Tot accum_t (decreases idx)
-   let rec _foldl__loop (item_t: Type) (accum_t: Type) seq fn accum idx 
-      = 
-         if idx = 0 then
+      #item_t: Type 
+      -> #accum_t: Type 
+      -> seq: seq_g item_t 
+      -> (accum_t -> index_g seq -> Tot accum_t) 
+      -> accum_t 
+      -> index: index_g seq
+      -> Tot accum_t (decreases index)
+   let rec _foldl__loop (item_t: Type) (accum_t: Type) seq fold accum index 
+      =  if index = 0 then
             accum
          else
-            _foldl__loop seq fn (fn accum (nth seq idx)) (idx - 1)
+            _foldl__loop seq fold (fold accum index) (index - 1)
+
+   val _foldl: 
+      #item_t: Type 
+      -> #accum_t: Type 
+      -> seq: seq_g item_t 
+      -> (accum_t -> index_g seq -> Tot accum_t) 
+      -> accum_t 
+      -> Tot accum_t
+   let rec _foldl (item_t: Type) (accum_t: Type) seq fold accum 
+      =  let len = length seq in
+         if len = 0 then
+            accum
+         else
+            _foldl__loop seq fold accum (len - 1)
 
    val foldl: 
-      #item_t: Type -> #accum_t: Type 
-      -> (accum_t -> item_t -> Tot accum_t) -> accum_t -> seq_g item_t 
+      #item_t: Type 
+      -> #accum_t: Type 
+      -> (accum_t -> item_t -> Tot accum_t) 
+      -> accum_t 
+      -> seq_g item_t 
       -> Tot accum_t
-   let rec foldl (item_t: Type) (accum_t: Type) fn accum seq 
-      = 
-         let len = length seq in
-            if 0 = len then
-               accum
-            else
-               _foldl__loop seq fn accum (len - 1)
+   let rec foldl (item_t: Type) (accum_t: Type) fold accum seq 
+      =  let len = length seq in
+         let adaptor  = (fun accum index -> fold accum (nth seq index)) in
+         _foldl seq adaptor accum 
 
    val filter: 
       #item_t: Type
       -> (item_t -> Tot bool)
       -> seq_g item_t 
       -> Tot (seq_g item_t)
-   let filter (item_t: Type) fn seq 
-      =
-         foldl
-            (fun (a: seq_g item_t) e ->
-               if fn e then
-                  append a e
-               else
-                  a)
-            Seq.empty
+   let filter (item_t: Type) pred seq 
+      =  _foldl
             seq
+            (fun (accum: seq_g item_t) index ->
+               let item = nth seq index in
+                  if pred item then
+                     append accum item
+                  else
+                     accum)
+            empty
 
    val map:
       #item0_t: Type
@@ -203,12 +220,57 @@ module Tesseract.Specs.Seq
       -> (item0_t -> Tot item1_t)
       -> seq_g item0_t
       -> Tot (seq_g item1_t)
-   let map (item0_t: Type) (item1_t: Type) fn seq0
-      = 
-         foldl
-            (fun (accum: seq_g item1_t) item ->
-               Seq.append accum (fn item))
-            Seq.empty
+   let map (item0_t: Type) (item1_t: Type) xform seq0
+      =  _foldl
             seq0
+            (fun (accum: seq_g item1_t) index ->
+               append accum (xform (nth seq0 index)))
+            empty
+
+   val maybe_find:
+      #item_t: Type
+      -> (item_t -> Tot bool)
+      -> seq: seq_g item_t
+      -> index_g seq
+      -> Tot (option nat)
+   let maybe_find (item_t: Type) pred seq start
+      =  _foldl
+            seq
+            (fun (accum: option nat) index ->
+               if index >= start then
+                  match accum with
+                     | None ->
+                        if pred (nth seq index) then
+                           Some index
+                        else
+                           accum
+                     | _ ->
+                        accum
+               else
+                  accum)
+            None
+
+   val find:
+      #item_t: Type
+      -> pred: (item_t -> Tot bool)
+      -> seq: seq_g item_t
+      -> start: index_g seq{is_Some (maybe_find pred seq start)}
+      -> Tot (option nat)
+   let find (item_t: Type) pred seq start
+      =  _foldl
+            seq
+            (fun (accum: option nat) index ->
+               if index >= start then
+                  match accum with
+                     | None ->
+                        if pred (nth seq index) then
+                           Some index
+                        else
+                           accum
+                     | _ ->
+                        accum
+               else
+                  accum)
+            None
 
 // $vim-fst:32: vim:set sts=3 sw=3 et ft=fstar:,$
